Challenge/Ripemd160/Submission/Proofs/Bytecode/StackRoundData.lean
@@ -61,18 +61,18 @@ def rightConstant (i : Nat) : UInt256 :=
 def leftHelperPCOfGroup (group : Nat) : UInt256 :=
   match group with
   | 0 => UInt256.ofNat 0xfca
-  | 1 => UInt256.ofNat 0x1001
-  | 2 => UInt256.ofNat 0x1040
-  | 3 => UInt256.ofNat 0x107e
-  | _ => UInt256.ofNat 0x10bd
+  | 1 => UInt256.ofNat 0xffe
+  | 2 => UInt256.ofNat 0x103a
+  | 3 => UInt256.ofNat 0x1075
+  | _ => UInt256.ofNat 0x10b1
 
 def rightHelperPCOfGroup (group : Nat) : UInt256 :=
   match group with
-  | 0 => UInt256.ofNat 0x10fb
-  | 1 => UInt256.ofNat 0x1139
-  | 2 => UInt256.ofNat 0x1178
-  | 3 => UInt256.ofNat 0x11b6
-  | _ => UInt256.ofNat 0x11f5
+  | 0 => UInt256.ofNat 0x10ec
+  | 1 => UInt256.ofNat 0x1127
+  | 2 => UInt256.ofNat 0x1163
+  | 3 => UInt256.ofNat 0x119e
+  | _ => UInt256.ofNat 0x11da
 
 def leftHelperPC (i : Nat) : UInt256 :=
   leftHelperPCOfGroup (i / 16)
@@ -82,7 +82,7 @@ def rightHelperPC (i : Nat) : UInt256 :=
 
 def wrapperTemplate (returnPC xAddress helperPC : UInt256)
     (rotation : Nat) : List Instr :=
-  [push1 (UInt256.ofNat rotation), push2 returnPC, push2 xAddress,
+  [push1 (UInt256.ofNat (32 - rotation)), push2 returnPC, push2 xAddress,
     push2 helperPC, op .JUMP, op .JUMPDEST]
 
 def leftTemplate (i : Nat) : List Instr :=
